src/PredCalc/NAryEquivLemmas.v
@@ -1,0 +1,761 @@
+From Equations Require Import Equations.
+From Stdlib Require Import Lia.
+From Stdlib Require Import Lists.List.
+From stdpp Require Import base list_monad sets gmap.
+From MRC Require Import Prelude.
+From MRC Require Import Stdppp.
+From MRC Require Import Model.
+From MRC Require Import SeqNotation.
+From MRC Require Import PredCalc.Basic.
+From MRC Require Import PredCalc.Equiv.
+From MRC Require Import PredCalc.SyntacticFacts.
+From MRC Require Import PredCalc.SemanticFacts.
+From MRC Require Import PredCalc.EquivLemmas.
+From MRC Require Import PredCalc.NAry.
+
+
+Section n_ary_lemmas.
+  Context {M : model}.
+
+  Local Notation value := (value M).
+  Local Notation term := (term value).
+  Local Notation atomic_formula := (atomic_formula value).
+  Local Notation formula := (formula value).
+
+  Implicit Types x y : variable.
+  Implicit Types t : term.
+  Implicit Types af : atomic_formula.
+  Implicit Types A B : formula.
+  Implicit Types xs : list variable.
+  Implicit Types ts : list term.
+  Implicit Types Bs Cs Ds : list formula.
+  Implicit Types vs : list value.
+
+  Lemma simpl_feval_and_list σ Bs :
+    feval σ <! ∧* Bs !> ↔ ∀ B, B ∈ Bs → feval σ B.
+  Proof with auto.
+    split.
+    - intros ? B' ?. induction Bs as [|B BS IH]; [set_solver|]. simpl in H. simp feval in H.
+      destruct H as []. apply elem_of_cons in H0 as [|].
+      + subst...
+      + apply IH...
+    - induction Bs as [|B BS IH]; [set_solver|]. simpl. simp feval. split.
+      + apply H. set_unfold. left...
+      + apply IH. intros B' ?. apply H. set_unfold. right...
+  Qed.
+
+  Lemma simpl_feval_or_list σ Bs :
+    feval σ <! ∨* Bs !> ↔ ∃ B, B ∈ Bs ∧ feval σ B.
+  Proof with auto.
+    split; intros.
+    - induction Bs as [|B BS IH]; [set_solver|]. simpl in H. simp feval in H. destruct H as [|].
+      + exists B. set_solver.
+      + apply IH in H as [B' HB]. exists B'. set_solver.
+    - destruct H as (B'&?&?). induction Bs as [|B Bs IH]; [set_solver|]. simpl.
+      simp feval. apply elem_of_cons in H as [|].
+      + subst. left...
+      + right. apply IH...
+  Qed.
+
+  Lemma simpl_feval_exists_list σ xs A :
+    feval σ <! ∃* xs, A !> ↔
+    ∃ vs (H : OfSameLength xs vs),
+      feval σ (@seq_subst _ A xs (TConst <$> vs) of_same_length_fmap_r).
+  Proof with auto.
+    split; intros.
+    - generalize dependent σ. induction xs as [|x xs IH]; simpl in *; intros.
+      + exists [], (of_same_length_nil). simpl...
+      + simp feval in H. destruct H as [v Hv]. rewrite feval_subst with (v:=v) in Hv...
+        apply IH in Hv as (vs&Hl&?). exists (v :: vs), of_same_length_cons.
+        simpl. rewrite feval_subst with (v:=v)...
+        eapply feval_proper; [reflexivity| | apply H]. apply seq_subst_proper... reflexivity.
+    - generalize dependent σ. induction xs as [|x xs' IH]; intros.
+      + destruct H as (vs&Hl&?). apply of_same_length_nil_inv_l in Hl as ?. subst. simpl in H...
+      + destruct H as (vs&Hl&?). apply of_same_length_cons_inv_l in Hl as ?.
+        destruct H0 as (v&vs'&?&?). subst. simpl. simp feval.
+        simpl in H. rewrite feval_subst with (v:=v) in H... exists v.
+        rewrite feval_subst with (v:=v)... apply IH. exists vs'.
+        apply of_same_length_rest in Hl as ?. exists H0.
+        eapply feval_proper; [reflexivity| | apply H]. apply seq_subst_proper... reflexivity.
+  Qed.
+
+
+  Lemma simpl_feval_forall_list σ xs A :
+    feval σ <! ∀* xs, A !> ↔
+    ∀ vs (H : OfSameLength xs vs),
+      feval σ (@seq_subst _ A xs (TConst <$> vs) of_same_length_fmap_r).
+  Proof with auto.
+    split; intros.
+    - generalize dependent σ. generalize dependent vs.
+      induction xs as [|x xs IH]; simpl in *; intros.
+      + apply of_same_length_nil_inv_l in H0 as ?. subst. simpl in H...
+      + apply of_same_length_cons_inv_l in H0 as ?.
+        destruct H1 as (v&vs'&?&?). subst. simpl. rewrite feval_subst with (v:=v)...
+        rewrite simpl_feval_fforall in H. specialize (H v).
+        rewrite feval_subst with (v:=v) in H...
+        apply (IH vs' (@of_same_length_rest _ _ _ _ _ _ H0)) in H.
+        eapply feval_proper; [reflexivity| | apply H]. apply seq_subst_proper... reflexivity.
+    - generalize dependent σ. induction xs as [|x xs IH]; simpl in *; intros.
+      + specialize (H [] of_same_length_nil). simpl in H...
+      + rewrite simpl_feval_fforall. intros. rewrite feval_subst with (v:=v)...
+        (* TODO: maybe rename fforall in [simpl_feval_fforall] to forall? *)
+        apply IH. intros. specialize (H (v::vs) (of_same_length_cons)). simpl in H.
+        rewrite feval_subst with (v:=v) in H...
+        eapply feval_proper; [reflexivity| | apply H]. apply seq_subst_proper... reflexivity.
+  Qed.
+
+  Lemma f_and_list_elim B Bs :
+    B ∈ Bs →
+    <! ∧* Bs !> ⇛ B.
+  Proof with auto.
+    intros. intros σ Hand. rewrite simpl_feval_and_list in Hand. apply Hand...
+  Qed.
+
+  Lemma f_or_list_intro B Bs :
+    B ∈ Bs →
+    B ⇛ <! ∨* Bs !>.
+  Proof with auto.
+    intros. intros σ HB. apply simpl_feval_or_list. exists B. split...
+  Qed.
+
+  Lemma f_and_absorb A B :
+    <! A ∧ (A ∨ B) !> ≡ A.
+  Proof. prove_equiv. Qed.
+
+  Lemma f_or_absorb A B :
+    <! A ∨ (A ∧ B) !> ≡ A.
+  Proof. prove_equiv. Qed.
+
+  Lemma f_and_or_distr A B C :
+    <! A ∧ (B ∨ C) !> ≡ <! (A ∧ B) ∨ (A ∧ C) !>.
+  Proof. prove_equiv. Qed.
+
+  Lemma f_or_and_distr A B C :
+    <! A ∨ (B ∧ C) !> ≡ <! (A ∨ B) ∧ (A ∨ C) !>.
+  Proof. prove_equiv. Qed.
+
+  Lemma f_and_true A :
+    <! A ∧ true !> ≡ A.
+  Proof. prove_equiv. Qed.
+
+  Lemma f_or_true A :
+    <! A ∨ true !> ≡ <! true !>.
+  Proof. prove_equiv. Qed.
+
+  Lemma f_and_false A :
+    <! A ∧ false !> ≡ <! false !>.
+  Proof. prove_equiv. Qed.
+
+  Lemma f_or_false A :
+    <! A ∨ false !> ≡ <! A !>.
+  Proof. prove_equiv. Qed.
+
+  Lemma f_not_true : <! ¬ true !> ≡@{formula} <! false !>.
+  Proof. prove_equiv. Qed.
+
+  Lemma f_not_false : <! ¬ false !> ≡@{formula} <! true !>.
+  Proof. prove_equiv. Qed.
+
+  Lemma f_and_not_self A :
+    <! A ∧ ¬ A !> ≡ <! false !>.
+  Proof. prove_equiv. Qed.
+
+  Lemma f_excluded_middle A :
+      <! A ∨ ¬ A !> ≡ <! true !>.
+  Proof. prove_equiv. Qed.
+
+  Lemma f_not_stable A :
+    <! ¬ ¬ A !> ≡ <! A !>.
+  Proof. prove_equiv. Qed.
+
+  Lemma f_not_and A B :
+    <! ¬ (A ∧ B) !> ≡ <! ¬ A ∨ ¬ B !>.
+  Proof. prove_equiv. Qed.
+
+  Lemma f_not_or A B :
+      <! ¬ (A ∨ B) !> ≡ <! ¬ A ∧ ¬ B !>.
+  Proof. prove_equiv. Qed.
+
+  Lemma f_or_not_absorb A B :
+      <! A ∨ (¬ A ∧ B) !> ≡ <! A ∨ B !>.
+  Proof. prove_equiv. Qed.
+
+  Lemma f_and_not_absorb A B :
+    <! A ∧ (¬ A ∨ B) !> ≡ <! A ∧ B !>.
+  Proof. prove_equiv. Qed.
+
+  (* A.22 *)
+  Lemma f_imp_equiv_or A B :
+    <! A ⇒ B !> ≡ <! ¬ A ∨ B !>.
+  Proof. prove_equiv. Qed.
+
+  (* A.23 *)
+  Lemma f_implies_self A :
+    <! A ⇒ A !> ≡ <! true !>.
+  Proof. prove_equiv. Qed.
+
+  (* A.24 *)
+  Lemma f_impl_as_not_and A B :
+    <! A ⇒ B !> ≡ <! ¬ (A ∧ ¬ B) !>.
+  Proof. prove_equiv. Qed.
+
+  (* A.25 *)
+  Lemma f_not_impl A B :
+      <! ¬ (A ⇒ B) !> ≡ <! A ∧ ¬ B !>.
+  Proof. prove_equiv. Qed.
+
+  (* A.26 *)
+  Lemma f_contrapositive A B :
+      <! A ⇒ B !> ≡ <! ¬ B ⇒ ¬ A !>.
+  Proof. prove_equiv. Qed.
+
+  (* A.27 *)
+  Lemma f_implies_true A :
+    <! A ⇒ true !> ≡ <! true !>.
+  Proof. prove_equiv. Qed.
+
+  (* A.28 *)
+  Lemma f_true_implies A :
+      <! true ⇒ A !> ≡ <! A !>.
+  Proof. prove_equiv. Qed.
+
+  (* A.29 *)
+  Lemma f_implies_false A :
+    <! A ⇒ false !> ≡ <! ¬ A !>.
+  Proof. prove_equiv. Qed.
+
+  (* A.30 *)
+  Lemma f_false_implies A :
+      <! false ⇒ A !> ≡ <! true !>.
+  Proof. prove_equiv. Qed.
+
+  (* A.31 *)
+  Lemma f_implies_not_self A :
+      <! A ⇒ ¬ A !> ≡ <! ¬ A !>.
+  Proof. prove_equiv. Qed.
+
+  (* A.32 *)
+  Lemma f_not_implies_self A :
+      <! ¬ A ⇒ A !> ≡ <! A !>.
+  Proof. prove_equiv. Qed.
+
+  (* A.33 *)
+  Lemma f_impl_and_r A B C :
+      <! C ⇒ (A ∧ B) !> ≡ <! (C ⇒ A) ∧ (C ⇒ B) !>.
+  Proof. prove_equiv. Qed.
+
+  (* A.34 *)
+  Lemma f_impl_or_l A B C :
+    <! (A ∨ B) ⇒ C !> ≡ <! (A ⇒ C) ∧ (B ⇒ C) !>.
+  Proof. prove_equiv. Qed.
+
+  (* A.35 *)
+  Lemma f_impl_or_r A B C :
+    <! C ⇒ (A ∨ B) !> ≡ <! (C ⇒ A) ∨ (C ⇒ B) !>.
+  Proof. prove_equiv. Qed.
+
+  (* A.36 *)
+  Lemma f_impl_and_l A B C :
+    <! (A ∧ B) ⇒ C !> ≡ <! (A ⇒ C) ∨ (B ⇒ C) !>.
+  Proof with auto.
+    unfold FImpl. intros σ. simp feval. split; [| naive_solver].
+    intros [|]... apply Decidable.not_and in H as [|]... apply feval_dec.
+  Qed.
+
+  (* A.37 *)
+  Lemma f_impl_curry A B C :
+    <! A ⇒ (B ⇒ C) !> ≡ <! (A ∧ B) ⇒ C !>.
+  Proof with auto.
+    unfold FImpl. intros σ. simp feval. split; [naive_solver |].
+    intros [|]... apply Decidable.not_and in H as [|]... apply feval_dec.
+  Qed.
+
+  (* A.38 *)
+  Lemma f_cases_as_or A B C :
+    <! (A ⇒ B) ∧ (¬A ⇒ C) !> ≡ <! (A ∧ B) ∨ (¬A ∧ C) !>.
+  Proof. prove_equiv. Qed.
+
+  (* A.39 *)
+  Lemma f_iff_as_and A B C :
+    <! A ⇔ B !> ≡ <! (A ⇒ B) ∧ (B ⇒ A) !>.
+  Proof. prove_equiv. Qed.
+
+  (* A.40 *)
+  Lemma f_iff_as_or A B :
+    <! A ⇔ B !> ≡ <! (A ∧ B) ∨ ¬(A ∨ B) !>.
+  Proof. prove_equiv. Qed.
+
+  (* A.41 *)
+  Lemma f_iff_negate A B :
+    <! A ⇔ B !> ≡ <! ¬A ⇔ ¬B !>.
+  Proof. prove_equiv. Qed.
+
+  (* A.42 *)
+  Lemma f_iff_self A :
+    <! A ⇔ A !> ≡ <! true !>.
+  Proof. prove_equiv. Qed.
+
+  (* A.43 *)
+  Lemma f_iff_not_self A :
+    <! A ⇔ ¬ A !> ≡ <! false !>.
+  Proof. prove_equiv. Qed.
+
+  (* A.44 *)
+  Lemma f_iff_true A :
+    <! A ⇔ true !> ≡ <! A !>.
+  Proof. prove_equiv. Qed.
+
+  (* A.45 *)
+  Lemma f_iff_false A :
+    <! A ⇔ false !> ≡ <! ¬ A !>.
+  Proof. prove_equiv. Qed.
+
+  (* A.46 *)
+  Lemma f_iff_and_absorb A B :
+    <! A ⇔ (A ∧ B) !> ≡ <! A ⇒ B !>.
+  Proof. prove_equiv. Qed.
+
+  (* A.47 *)
+  Lemma f_iff_or_absorb A B :
+    <! A ⇔ (A ∨ B) !> ≡ <! B ⇒ A !>.
+  Proof with auto.
+    intros σ. unfold FIff, FImpl. simp feval. split.
+    - intros []. destruct_or! H; naive_solver.
+    - intros [|]; [|naive_solver]. split.
+      + pose proof (feval_lem σ A). destruct H0 as [|]...
+      + pose proof (feval_lem σ A) as [|]; naive_solver.
+  Qed.
+
+  (* A.48 *)
+  Lemma f_or_iff A B C :
+    <! A ∨ (B ⇔ C) !> ≡ <! (A ∨ B) ⇔ (A ∨ C) !>.
+  Proof with auto.
+    intros σ. unfold FIff, FImpl. simp feval. split; [|naive_solver].
+    intros [|[]]; [naive_solver|]. split; destruct (feval_lem σ A); naive_solver.
+  Qed.
+
+  (* A.49 *)
+  Lemma f_iff_comm A B :
+    <! A ⇔ B !> ≡ <! B ⇔ A !>.
+  Proof. prove_equiv. Qed.
+
+  (* A.50 *)
+  Lemma f_iff_assoc A B C :
+      <! A ⇔ (B ⇔ C) !> ≡ <! (A ⇔ B) ⇔ C !>.
+  Proof.
+    unfold FIff, FImpl. rewrite f_not_and.
+    repeat rewrite f_not_and. repeat rewrite f_not_or. repeat rewrite f_not_stable.
+    intros σ. simp feval. split; naive_solver.
+  Qed.
+
+  (* A.56 *)
+  Lemma f_exists_one_point x t A :
+      x ∉ term_fvars t →
+      <! ∃ x, ⌜x = t⌝ ∧ A !> ≡ <! A[x \ t] !>.
+  Proof with auto.
+    intros Hfree σ. simp feval. setoid_rewrite simpl_subst_and.
+    setoid_rewrite simpl_subst_af. simpl. destruct (decide (x = x)); [|contradiction].
+    clear e. split.
+    - intros [v Hv]. simp feval in Hv. destruct Hv as [H1 H2]. inversion H1.
+      destruct H as []. inversion H. subst v0 x0. clear H H1.
+      (* TODO: teval_subst looks ugly match it with feval_subst *)
+      rewrite <- (@teval_subst _ _ _ _ _ v _) in H0...
+      apply teval_delete_state_var_head in H0... rewrite (feval_subst v)...
+      rewrite <- (feval_subst _ (TConst v))...
+    - intros. pose proof (teval_total σ t) as [v Hv]. exists v. simp feval. split.
+      + simpl. exists v. split... rewrite <- (@teval_subst _ _ _ _ _ v _)...
+        rewrite teval_delete_state_var_head...
+      + rewrite (feval_subst v) in H... rewrite (feval_subst v)...
+  Qed.
+
+  (* A.56 *)
+  Lemma f_forall_one_point x t A :
+      x ∉ term_fvars t →
+      <! ∀ x, ⌜x = t⌝ ⇒ A !> ≡ <! A[x \ t] !>.
+  Proof with auto.
+    intros Hfree. unfold FForall. rewrite f_not_impl.
+    apply (f_exists_one_point x t(FNot A)) in Hfree. rewrite Hfree.
+    rewrite simpl_subst_not. rewrite f_not_stable...
+  Qed.
+
+  (* A.60 *)
+  Lemma f_exists_idemp x A :
+    <! ∃ x x, A !> ≡ <! ∃ x, A !>.
+  Proof with auto. rewrite fexists_unused... simpl. set_solver. Qed.
+
+  (* A.59 *)
+  Lemma f_forall_idemp x A :
+    <! ∀ x x, A !> ≡ <! ∀ x, A !>.
+  Proof with auto. unfold FForall. rewrite f_not_stable. rewrite f_exists_idemp... Qed.
+
+  (* A.61 *)
+  Lemma f_not_forall x A :
+    <! ¬ ∀ x, A !> ≡ <! ∃ x, ¬ A !>.
+  Proof. unfold FForall. rewrite f_not_stable. auto. Qed.
+
+  (* A.62 *)
+  Lemma f_not_exists x A :
+    <! ¬ ∃ x, A !> ≡ <! ∀ x, ¬ A !>.
+  Proof. unfold FForall. rewrite f_not_stable. auto. Qed.
+
+  (* A.64 *)
+  Lemma f_exists_comm x y A :
+    <! ∃ x y, A !> ≡ <! ∃ y x, A !>.
+  Proof with auto.
+    intros σ. destruct (decide (x = y)). 1:{ subst... }
+    destruct (decide (x ∈ formula_fvars A)).
+    2:{ rewrite fexists_unused.
+        - rewrite (fexists_unused x)...
+        - simpl. set_solver. }
+    destruct (decide (y ∈ formula_fvars A)).
+    2:{ rewrite (fexists_unused y)...
+        rewrite (fexists_unused y)... simpl. set_solver. }
+    simp feval. split.
+    - intros [vx H]. rewrite (feval_subst vx) in H... simp feval in H. destruct H as [vy H].
+      rewrite (feval_subst vy) in H... exists vy. rewrite (feval_subst vy)...
+      simp feval. exists vx. rewrite (feval_subst vx)... rewrite (insert_commute σ)...
+    - intros [vy H]. rewrite (feval_subst vy) in H... simp feval in H. destruct H as [vx H].
+      rewrite (feval_subst vx) in H... exists vx. rewrite (feval_subst vx)...
+      simp feval. exists vy. rewrite (feval_subst vy)... rewrite (insert_commute σ)...
+  Qed.
+
+  (* A.63 *)
+  Lemma f_forall_comm x y A :
+    <! ∀ x y, A !> ≡ <! ∀ y x, A !>.
+  Proof. unfold FForall. do 2 rewrite f_not_stable. rewrite f_exists_comm. reflexivity. Qed.
+
+  (* A.66 *)
+  Lemma f_exists_or x A B :
+    <! ∃ x, A ∨ B !> ≡ <! (∃ x, A) ∨ (∃ x, B) !>.
+  Proof with auto.
+    intros σ. simp feval. setoid_rewrite simpl_subst_or. split.
+    - intros [v H]. simp feval in H. destruct H as [|]; [left|right]; exists v...
+    - intros [[v H] | [v H]]; exists v; simp feval...
+  Qed.
+
+  (* A.65 *)
+  Lemma f_forall_and x A B :
+    <! ∀ x, A ∧ B !> ≡ <! (∀ x, A) ∧ (∀ x, B) !>.
+  Proof. unfold FForall. rewrite f_not_and. rewrite f_exists_or. rewrite f_not_or; auto. Qed.
+
+  (* A.67 *)
+  Lemma f_exists_impl x A B :
+    <! ∃ x, A ⇒ B !> ≡ <! (∀ x, A) ⇒ (∃ x, B) !>.
+  Proof with auto.
+    intros σ. unfold FImpl. rewrite f_exists_or. unfold FForall. rewrite f_not_stable...
+  Qed.
+
+  (* A.68 *)
+  Lemma f_forall_ent_exists x A :
+    <! ∀ x, A !> ⇛ <! ∃ x, A !>.
+  Proof.
+    intros σ. rewrite simpl_feval_fforall. intros. simp feval.
+    exists ⊥. apply H.
+  Qed.
+
+  (* A.69 *)
+  Lemma f_or_forall x A B :
+    <! (∀ x, A) ∨ (∀ x, B) !> ⇛ <! ∀ x, A ∨ B !>.
+  Proof.
+    intros σ. simp feval. do 3 rewrite simpl_feval_fforall.
+    setoid_rewrite simpl_subst_or.
+    intros [|]; intros; simp feval; naive_solver.
+  Qed.
+
+  (* A.70 *)
+  Lemma f_forall_impl x A B :
+    <! ∀ x, A ⇒ B !> ⇛ <! (∀ x, A) ⇒ (∀ x, B) !>.
+  Proof.
+    intros σ. rewrite simpl_feval_fimpl. do 3 rewrite simpl_feval_fforall.
+    intros. specialize (H v). rewrite simpl_subst_impl in H. rewrite simpl_feval_fimpl in H.
+    naive_solver.
+  Qed.
+
+  (* A.71 *)
+  Lemma f_exists_and x A B :
+    <! ∃ x, A ∧ B !> ⇛ <! (∃ x, A) ∧ (∃ x, B) !>.
+  Proof with auto.
+    intros σ. simp feval. intros [v H]. rewrite simpl_subst_and in H. simp feval in H.
+    destruct H as []. split; exists v...
+  Qed.
+
+  (* A.72 *)
+  Lemma f_impl_exists x A B :
+    <! (∃ x, A) ⇒ (∃ x, B) !> ⇛ <! ∃ x, A ⇒ B !>.
+  Proof with auto.
+    intros σ. rewrite simpl_feval_fimpl. intros. simp feval.
+    setoid_rewrite simpl_subst_impl. setoid_rewrite simpl_feval_fimpl.
+    destruct (feval_lem σ <! ∃ x, A !>).
+    - apply H in H0. simp feval in H0. destruct H0 as [v Hv]. exists v. intros...
+    - exists ⊥. intros. simp feval in H0. exfalso. apply H0. exists ⊥...
+  Qed.
+
+  (* A.73 *)
+  Lemma f_exists_forall x y A :
+    <! ∃ x, (∀ y, A) !> ⇛ <! ∀ y, (∃ x, A) !>.
+  Proof with auto.
+    intros σ. simp feval. rewrite simpl_feval_fforall. intros [vx H] vy.
+    destruct (decide (x = y)).
+    1:{ subst y. rewrite simpl_subst_forall_skip in H... rewrite simpl_subst_exists_skip...
+        apply f_forall_ent_exists in H... }
+    rewrite (feval_subst vx) in H... rewrite simpl_feval_fforall in H.
+    specialize (H vy). rewrite (feval_subst vy) in H...
+    rewrite (feval_subst vy)... simp feval. exists vx. rewrite (feval_subst vx)...
+    rewrite (insert_commute σ)...
+  Qed.
+
+  (* A.74: fforall_unused *)
+  (* A.75: fexists_unused *)
+
+  (* A.76 *)
+  Lemma f_forall_and_unused_l x A B :
+    x ∉ formula_fvars A →
+    <! ∀ x, A ∧ B !> ≡ <! A ∧ (∀ x, B) !>.
+  Proof with auto. intros. rewrite f_forall_and. rewrite fforall_unused... Qed.
+
+  (* A.76' *)
+  Lemma f_forall_and_unused_r x A B :
+    x ∉ formula_fvars B →
+    <! ∀ x, A ∧ B !> ≡ <! (∀ x, A) ∧ B !>.
+  Proof with auto. intros. rewrite f_forall_and. rewrite (fforall_unused x B)... Qed.
+
+  (* A.77 *)
+  Lemma f_forall_or_unused_l x A B :
+    x ∉ formula_fvars A →
+    <! ∀ x, A ∨ B !> ≡ <! A ∨ (∀ x, B) !>.
+  Proof with auto.
+    intros. intros σ. rewrite simpl_feval_fforall. setoid_rewrite simpl_subst_or.
+    split; intros.
+    - simp feval. destruct (feval_lem σ A)... right. rewrite simpl_feval_fforall.
+      intros. specialize (H0 v). simp feval in H0. destruct H0...
+      rewrite (feval_subst v) in H0... apply feval_delete_state_var_head in H0...
+      contradiction.
+    - simp feval in *. rewrite (feval_subst v)... rewrite feval_delete_state_var_head...
+      destruct H0... right. rewrite simpl_feval_fforall in H0. apply H0.
+  Qed.
+
+  (* A.77' *)
+  Lemma f_forall_or_unused_r x A B :
+    x ∉ formula_fvars B →
+    <! ∀ x, A ∨ B !> ≡ <! (∀ x, A) ∨ B !>.
+  Proof with auto.
+    intros. intros σ. rewrite simpl_feval_fforall. setoid_rewrite simpl_subst_or.
+    split; intros.
+    - simp feval. destruct (feval_lem σ B)... left. rewrite simpl_feval_fforall.
+      intros. specialize (H0 v). simp feval in H0. destruct H0...
+      rewrite (feval_subst v) in H0... apply feval_delete_state_var_head in H0...
+      contradiction.
+    - simp feval in *. destruct H0.
+      + left. rewrite simpl_feval_fforall in H0. apply H0...
+      + right. rewrite (feval_subst v)... rewrite feval_delete_state_var_head...
+  Qed.
+
+  (* A.78 *)
+  Lemma f_forall_impl_unused_l x A B :
+    x ∉ formula_fvars A →
+    <! ∀ x, A ⇒ B !> ≡ <! A ⇒ (∀ x, B) !>.
+  Proof with auto.
+    intros. intros σ. rewrite simpl_feval_fforall. setoid_rewrite simpl_subst_impl.
+    rewrite simpl_feval_fimpl.
+    split; intros.
+    - rewrite simpl_feval_fforall. intros. specialize (H0 v). rewrite simpl_feval_fimpl in H0.
+      rewrite (feval_subst v) in H0... rewrite feval_delete_state_var_head in H0...
+    - rewrite simpl_feval_fimpl. intros. rewrite (feval_subst v) in H1...
+      rewrite feval_delete_state_var_head in H1... apply H0 in H1.
+      rewrite simpl_feval_fforall in H1...
+  Qed.
+
+  (* A.79 *)
+  Lemma f_forall_impl_unused_r x A B :
+    x ∉ formula_fvars B →
+    <! ∀ x, A ⇒ B !> ≡ <! (∃ x, A) ⇒ B !>.
+  Proof with auto.
+    intros. intros σ. rewrite simpl_feval_fforall. setoid_rewrite simpl_subst_impl.
+    setoid_rewrite simpl_feval_fimpl. simp feval.
+    split; intros.
+    - destruct H1 as [v Hv]. apply H0 in Hv. apply (feval_subst v) in Hv...
+      apply feval_delete_state_var_head in Hv...
+    - forward H0 by (exists v)... apply (feval_subst v)... apply feval_delete_state_var_head...
+  Qed.
+
+  (* A.80 *)
+  Lemma f_exists_and_unused_l x A B :
+    x ∉ formula_fvars A →
+    <! ∃ x, A ∧ B !> ≡ <! A ∧ (∃ x, B) !>.
+  Proof with auto.
+    intros. rewrite <- (f_not_stable A). rewrite <- (f_not_stable B). rewrite <- (f_not_or).
+    rewrite <- (f_not_forall). rewrite f_forall_or_unused_l by (simpl; auto).
+    rewrite f_not_or. rewrite f_not_forall...
+  Qed.
+
+  (* A.80' *)
+  Lemma f_exists_and_unused_r x A B :
+    x ∉ formula_fvars B →
+    <! ∃ x, A ∧ B !> ≡ <! (∃ x, A) ∧ B !>.
+  Proof with auto.
+    intros. rewrite <- (f_not_stable A). rewrite <- (f_not_stable B). rewrite <- (f_not_or).
+    rewrite <- (f_not_forall). rewrite f_forall_or_unused_r by (simpl; auto).
+    rewrite f_not_or. rewrite f_not_forall...
+  Qed.
+
+  (* A.81 *)
+  Lemma f_exists_or_unused_l x A B :
+    x ∉ formula_fvars A →
+    <! ∃ x, A ∨ B !> ≡ <! A ∨ (∃ x, B) !>.
+  Proof with auto. intros. rewrite f_exists_or. rewrite fexists_unused... Qed.
+
+  (* A.81' *)
+  Lemma f_exists_or_unused_r x A B :
+    x ∉ formula_fvars B →
+    <! ∃ x, A ∨ B !> ≡ <! (∃ x, A) ∨ B !>.
+  Proof with auto. intros. rewrite f_exists_or. rewrite (fexists_unused _ B)... Qed.
+
+  (* A.82 *)
+  Lemma f_exists_impl_unused_l x A B :
+    x ∉ formula_fvars A →
+    <! ∃ x, A ⇒ B !> ≡ <! A ⇒ (∃ x, B) !>.
+  Proof with auto. intros. rewrite f_exists_impl. rewrite fforall_unused... Qed.
+
+  (* A.83 *)
+  Lemma f_exists_impl_unused_r x A B :
+    x ∉ formula_fvars B →
+    <! ∃ x, A ⇒ B !> ≡ <! (∀ x, A) ⇒ B !>.
+  Proof with auto. intros. rewrite f_exists_impl. rewrite fexists_unused... Qed.
+
+  (* A.84: fforall_alpha_equiv *)
+  (* A.85: fexists_alpha_equiv *)
+
+  (* A.86 *)
+  Lemma f_forall_elim t x A :
+    <! ∀ x, A !> ⇛ <! A[x \ t] !>.
+  Proof with auto.
+    intros σ. rewrite simpl_feval_fforall. intros. pose proof (teval_total σ t) as [v Hv].
+    specialize (H v). rewrite (feval_subst v) in H... rewrite (feval_subst v)...
+  Qed.
+
+  (* A.86 *)
+  Lemma f_exists_intro t x A :
+    <! A[x \ t] !> ⇛ <! ∃ x, A !>.
+  Proof with auto.
+    intros σ. simp feval. intros. pose proof (teval_total σ t) as [v Hv].
+    exists v. rewrite (feval_subst v) in H... rewrite (feval_subst v)...
+  Qed.
+
+  Lemma f_impl_elim A B :
+    <! A ∧ (A ⇒ B) !> ⇛ B.
+  Proof with auto.
+    intros σ. simp feval. rewrite simpl_feval_fimpl. naive_solver.
+  Qed.
+
+  (* some lemmas for proving equivalences and entailments *)
+
+  Lemma f_and_cancel_l A B C :
+    B ≡ C → <! A ∧ B !> ≡ <! A ∧ C !>.
+  Proof. intros. rewrite H. reflexivity. Qed.
+
+  Lemma f_and_cancel_r A B C :
+    B ≡ C → <! B ∧ A !> ≡ <! C ∧ A !>.
+  Proof. intros. rewrite H. reflexivity. Qed.
+
+  Lemma f_or_cancel_l A B C :
+    B ≡ C → <! A ∨ B !> ≡ <! A ∨ C !>.
+  Proof. intros. rewrite H. reflexivity. Qed.
+
+  Lemma f_or_cancel_r A B C :
+    B ≡ C → <! B ∨ A !> ≡ <! C ∨ A !>.
+  Proof. intros. rewrite H. reflexivity. Qed.
+
+  Lemma f_impl_cancel_l A B C :
+    B ≡ C → <! A ⇒ B !> ≡ <! A ⇒ C !>.
+  Proof. intros. rewrite H. reflexivity. Qed.
+
+  Lemma f_impl_cancel_r A B C :
+    B ≡ C → <! B ⇒ A !> ≡ <! C ⇒ A !>.
+  Proof. intros. rewrite H. reflexivity. Qed.
+
+  Lemma f_subst_cancel A B x t :
+    A ≡ B → <! A[x \ t] !> ≡ <! B[x \ t] !>.
+  Proof. intros. rewrite H. reflexivity. Qed.
+
+  Lemma f_subst_cancel_term A x t1 t2 :
+    t1 ≡ t2 → <! A[x \ t1] !> ≡ <! A[x \ t2] !>.
+  Proof. intros. rewrite H. reflexivity. Qed.
+
+  Lemma f_exists_equiv A B y1 y2 :
+    (∀ t, <! A[y1 \ t] !> ≡ <! B[y2 \ t] !>) →
+    <! ∃ y1, A !> ≡ <! ∃ y2, B !>.
+  Proof. intros Hequiv σ. apply feval_exists_equiv_if. naive_solver. Qed.
+
+  Lemma f_forall_equiv A B y1 y2 :
+    (∀ t, <! A[y1 \ t] !> ≡ <! B[y2 \ t] !>) →
+    <! ∀ y1, A !> ≡ <! ∀ y2, B !>.
+  Proof. intros Hequiv σ. do 2 rewrite simpl_feval_fforall. naive_solver. Qed.
+
+  Lemma f_ent_and_cancel_l A B C :
+    B ⇛ C → <! A ∧ B !> ⇛ <! A ∧ C !>.
+  Proof. intros H σ. simp feval. specialize (H σ). naive_solver. Qed.
+
+  Lemma f_ent_and_cancel_r A B C :
+    B ⇛ C → <! B ∧ A !> ⇛ <! C ∧ A !>.
+  Proof. intros H σ. simp feval. specialize (H σ). naive_solver. Qed.
+
+  Lemma f_ent_or_cancel_l A B C :
+    B ⇛ C → <! A ∨ B !> ⇛ <! A ∨ C !>.
+  Proof. intros H σ. simp feval. specialize (H σ). naive_solver. Qed.
+
+  Lemma f_ent_or_cancel_r A B C :
+    B ⇛ C → <! B ∨ A !> ⇛ <! C ∨ A !>.
+  Proof. intros H σ. simp feval. specialize (H σ). naive_solver. Qed.
+
+  Lemma f_ent_subst_cancel A B x t :
+    A ⇛ B → <! A[x \ t] !> ⇛ <! B[x \ t] !>.
+  Proof with auto.
+    intros Hent σ H. pose proof (teval_total σ t) as [v Hv]. rewrite (feval_subst v) in H...
+    apply Hent in H. rewrite (feval_subst v)...
+  Qed.
+
+  Lemma f_ent_impl_cancel_l A B C :
+    B ⇛ C → <! A ⇒ B !> ⇛ <! A ⇒ C !>.
+  Proof. intros H σ. do 2 rewrite simpl_feval_fimpl. naive_solver. Qed.
+
+  Lemma f_ent_impl_cancel_r A B C :
+    C ⇛ B → <! B ⇒ A !> ⇛ <! C ⇒ A !>.
+  Proof. intros H σ. do 2 rewrite simpl_feval_fimpl. naive_solver. Qed.
+
+  Lemma f_exists_ent A B y1 y2 :
+    (∀ t, <! A[y1 \ t] !> ⇛ <! B[y2 \ t] !>) →
+    <! ∃ y1, A !> ⇛ <! ∃ y2, B !>.
+  Proof.
+    intros Hequiv σ. simp feval. intros [v Hv]. exists v. naive_solver.
+  Qed.
+
+  Lemma f_forall_ent A B y1 y2 :
+    (∀ t, <! A[y1 \ t] !> ⇛ <! B[y2 \ t] !>) →
+    <! ∀ y1, A !> ⇛ <! ∀ y2, B !>.
+  Proof.
+    intros Hequiv σ. do 2 rewrite simpl_feval_fforall. intros. naive_solver.
+  Qed.
+
+  Lemma f_ent_elim σ A B :
+    feval σ A →
+    A ⇛ B →
+    feval σ B.
+  Proof. naive_solver. Qed.
+
+  Lemma f_ent_intro A B :
+    (∀ σ, feval σ A → feval σ B) →
+    A ⇛ B.
+  Proof. naive_solver. Qed.
+
+  Lemma f_eq_refl t :
+    <! ⌜t = t⌝ !> ≡ <! true !>.
+  Proof.
+    prove_equiv. intros. destruct (teval_total σ t) as [v Hv]. econstructor. split; exact Hv.
+  Qed.
+
+  Lemma f_neq_irrefl t :
+    <! ⌜t ≠ t⌝ !> ≡ <! false !>.
+  Proof.
+    rewrite f_eq_refl. rewrite f_not_true. reflexivity.
+  Qed.
+End n_ary_lemmas.
